src/Tree_stack.thy
@@ -1,3 +1,4 @@
+(* [[file:~/workspace/agenda/myTasks.org::tree_stack_src][tree_stack_src]] *)
 theory Tree_stack
 imports Tree
 begin
@@ -11,8 +12,14 @@ type_synonym left_bound = "key option"
 
 type_synonym right_bound = "key option"
 
-type_synonym context_t = "(left_bound * (node_t * nat) * right_bound) list"
+type_synonym context_t =
+ "(left_bound * (node_t * nat) * right_bound) list"
 (*end context definition*)
+
+definition ctx_to_map :: "context_t => (key,value_t) map" where
+"ctx_to_map ctx == (
+let leaves = List.map (% (_,(n,_),_). List.concat(tree_to_leaves (Node(n)))) ctx in
+map_of(List.concat leaves))"
 
 (*begin treestack definition*)
 datatype 'f tree_stack = Tree_stack "'f focus_t * context_t"
@@ -23,25 +30,32 @@ definition subtree_indexes :: "node_t => nat set" where
 "subtree_indexes n == (
   case n of (l,_) =>  { 0 .. (length l)})"
 
-definition is_subnode :: "(node_t * nat) => (node_t * nat) => bool" where
-"is_subnode ni pi == (
-  let (n,_) = ni in
+definition is_subnode 
+ :: "node_t => (node_t * nat) => bool"
+where
+"is_subnode n pi == (
   let ((ks,rs),i) = pi in
   Node n = (rs!i))"
 
-fun linked_context :: "(left_bound * (node_t * nat) * right_bound) => context_t => bool" where
+fun linked_context 
+ :: "(left_bound * (node_t * nat) * right_bound) => context_t => bool"
+where
 "linked_context ni [] = True" |
-"linked_context (lb,ni,rb) ((plb,pi,prb)#pis) = (
-  is_subnode ni pi & linked_context (plb,pi,prb) pis)"
+"linked_context (lb,(n,i),rb) ((plb,pi,prb)#pis) = (
+  is_subnode n pi & linked_context (plb,pi,prb) pis)"
 
-definition get_lower_upper_keys_for_node_t :: "key list => left_bound => nat => right_bound => (key option * key option)" where
+definition get_lower_upper_keys_for_node_t
+ :: "key list => left_bound => nat => right_bound => (key option * key option)"
+where
 "get_lower_upper_keys_for_node_t ls lb i rb == (
 let l = if (i = 0) then lb else Some(ls ! (i - 1))     in
 let u = if (i = (length ls)) then rb else Some(ls ! i) in
 (l,u)
 )"
 
-definition wellformed_context_1 :: "ms_t => (left_bound * (node_t * nat) * right_bound) => bool " where
+definition wellformed_context_1
+ :: "ms_t => (left_bound * (node_t * nat) * right_bound) => bool "
+where
 "wellformed_context_1 ms lbnirb == (
 let (lb,((ls,cs),i),rb) = lbnirb in
 let (l,u) = get_lower_upper_keys_for_node_t ls lb i rb  in
@@ -76,6 +90,8 @@ wellformed_context_1 None x1
 (*end wfcontext definition*)
 
 
-definition dest_ts :: "'f tree_stack \<Rightarrow> 'f * context_t" where
-"dest_ts ts == (case ts of Tree_stack((Focus f),c) \<Rightarrow> (f,c))"
+definition dest_ts :: "'f tree_stack => 'f * context_t" where
+"dest_ts ts == (case ts of Tree_stack((Focus f),c) => (f,c))"
+
 end
+(* tree_stack_src ends here *)
