src/Key_value.thy
@@ -5,6 +5,7 @@ begin
 typedecl key
 typedecl value_t
 
+(*begin key order operators definition*)
 consts key_lt :: "key => key => bool"
 
 definition key_eq :: "key => key => bool" where
@@ -12,12 +13,15 @@ definition key_eq :: "key => key => bool" where
 
 definition key_le :: "key => key => bool" where
   "key_le k1 k2 == (key_eq k1 k2) | (key_lt k1 k2)"
+(*end key order operators definition*)
 
 definition kv_lt :: "(key * value_t) => (key * value_t) => bool" where
   "kv_lt kv1 kv2 == (key_lt (fst kv1) (fst kv2))"
 
 (*begin check keys definition*)
-definition check_keys :: "key option => key list => key option => bool" where
+definition check_keys 
+ :: "key option => key list => key option => bool"
+where
 "check_keys kl ks kr == (
 let b1 = (
 case kl of None => True 
@@ -34,11 +38,12 @@ b1 & b2
 (*end check keys definition*)
 
 (*tr: assumes xs are sorted; returns list length if not found*)
+(*begin search key to index definition *)
 definition search_key_to_index :: "key list => key => nat" where
 "search_key_to_index ks k == (
 let num_keys = length ks in
 let index = List.find (% x. key_lt k (ks!x)) (upt 0 num_keys) in
 (case index of None => num_keys
 | Some x => x))"
-
+(*end search key to index definition *)
 end
